testdata/examples/semantics/semantics.gold.v
@@ -2997,12 +2997,18 @@ End def.
 
 End unit.
 
-Definition unitⁱᵐᵖˡ {ext : ffi_syntax} {go_gctx : GoGlobalContext} : go.type := go.StructType [
+Definition unit'fds_unsealed {ext : ffi_syntax} {go_gctx : GoGlobalContext} : list go.field_decl := [
+
 ].
+Program Definition unit'fds {ext : ffi_syntax} {go_gctx : GoGlobalContext} := sealed (unit'fds_unsealed).
+Global Instance equals_unfold_unit {ext : ffi_syntax} {go_gctx : GoGlobalContext} : unit'fds =→ unit'fds_unsealed.
+Proof. rewrite /unit'fds seal_eq //. Qed.
+
+Definition unitⁱᵐᵖˡ {ext : ffi_syntax} {go_gctx : GoGlobalContext} : go.type := go.StructType (unit'fds).
 
 Class unit_Assumptions {ext : ffi_syntax} `{!GoGlobalContext} `{!GoLocalContext} `{!GoSemanticsFunctions} : Prop :=
 {
-  #[global] unit_type_repr  :: go.TypeRepr unit unit.t;
+  #[global] unit_type_repr  :: go.TypeReprUnderlying unitⁱᵐᵖˡ unit.t;
   #[global] unit_underlying :: (unit) <u (unitⁱᵐᵖˡ);
 }.
 
@@ -3021,16 +3027,21 @@ End def.
 
 End Enc.
 
-Definition Encⁱᵐᵖˡ {ext : ffi_syntax} {go_gctx : GoGlobalContext} : go.type := go.StructType [
+Definition Enc'fds_unsealed {ext : ffi_syntax} {go_gctx : GoGlobalContext} : list go.field_decl := [
   (go.FieldDecl "p"%go (go.SliceType go.byte))
 ].
+Program Definition Enc'fds {ext : ffi_syntax} {go_gctx : GoGlobalContext} := sealed (Enc'fds_unsealed).
+Global Instance equals_unfold_Enc {ext : ffi_syntax} {go_gctx : GoGlobalContext} : Enc'fds =→ Enc'fds_unsealed.
+Proof. rewrite /Enc'fds seal_eq //. Qed.
+
+Definition Encⁱᵐᵖˡ {ext : ffi_syntax} {go_gctx : GoGlobalContext} : go.type := go.StructType (Enc'fds).
 
 Class Enc_Assumptions {ext : ffi_syntax} `{!GoGlobalContext} `{!GoLocalContext} `{!GoSemanticsFunctions} : Prop :=
 {
-  #[global] Enc_type_repr  :: go.TypeRepr Enc Enc.t;
+  #[global] Enc_type_repr  :: go.TypeReprUnderlying Encⁱᵐᵖˡ Enc.t;
   #[global] Enc_underlying :: (Enc) <u (Encⁱᵐᵖˡ);
-  #[global] Enc_get_p (x : Enc.t) :: go.IsGoStepPureDet (StructFieldGet (Enc) "p") #x #x.(Enc.p');
-  #[global] Enc_set_p (x : Enc.t) y :: go.IsGoStepPureDet (StructFieldSet (Enc) "p") (#x, #y) #(x <|Enc.p' := y|>);
+  #[global] Enc_get_p (x : Enc.t) :: ⟦StructFieldGet (Encⁱᵐᵖˡ) "p", #x⟧ ⤳[under] #x.(Enc.p');
+  #[global] Enc_set_p (x : Enc.t) y :: ⟦StructFieldSet (Encⁱᵐᵖˡ) "p", (#x, #y)⟧ ⤳[under] #(x <|Enc.p' := y|>);
   #[global] Enc'ptr_consume_unfold :: MethodUnfold (go.PointerType (Enc)) "consume" (Enc__consumeⁱᵐᵖˡ);
 }.
 
@@ -3049,16 +3060,21 @@ End def.
 
 End Dec.
 
-Definition Decⁱᵐᵖˡ {ext : ffi_syntax} {go_gctx : GoGlobalContext} : go.type := go.StructType [
+Definition Dec'fds_unsealed {ext : ffi_syntax} {go_gctx : GoGlobalContext} : list go.field_decl := [
   (go.FieldDecl "p"%go (go.SliceType go.byte))
 ].
+Program Definition Dec'fds {ext : ffi_syntax} {go_gctx : GoGlobalContext} := sealed (Dec'fds_unsealed).
+Global Instance equals_unfold_Dec {ext : ffi_syntax} {go_gctx : GoGlobalContext} : Dec'fds =→ Dec'fds_unsealed.
+Proof. rewrite /Dec'fds seal_eq //. Qed.
+
+Definition Decⁱᵐᵖˡ {ext : ffi_syntax} {go_gctx : GoGlobalContext} : go.type := go.StructType (Dec'fds).
 
 Class Dec_Assumptions {ext : ffi_syntax} `{!GoGlobalContext} `{!GoLocalContext} `{!GoSemanticsFunctions} : Prop :=
 {
-  #[global] Dec_type_repr  :: go.TypeRepr Dec Dec.t;
+  #[global] Dec_type_repr  :: go.TypeReprUnderlying Decⁱᵐᵖˡ Dec.t;
   #[global] Dec_underlying :: (Dec) <u (Decⁱᵐᵖˡ);
-  #[global] Dec_get_p (x : Dec.t) :: go.IsGoStepPureDet (StructFieldGet (Dec) "p") #x #x.(Dec.p');
-  #[global] Dec_set_p (x : Dec.t) y :: go.IsGoStepPureDet (StructFieldSet (Dec) "p") (#x, #y) #(x <|Dec.p' := y|>);
+  #[global] Dec_get_p (x : Dec.t) :: ⟦StructFieldGet (Decⁱᵐᵖˡ) "p", #x⟧ ⤳[under] #x.(Dec.p');
+  #[global] Dec_set_p (x : Dec.t) y :: ⟦StructFieldSet (Decⁱᵐᵖˡ) "p", (#x, #y)⟧ ⤳[under] #(x <|Dec.p' := y|>);
   #[global] Dec'ptr_consume_unfold :: MethodUnfold (go.PointerType (Dec)) "consume" (Dec__consumeⁱᵐᵖˡ);
 }.
 
@@ -3078,19 +3094,24 @@ End def.
 
 End Editor.
 
-Definition Editorⁱᵐᵖˡ {ext : ffi_syntax} {go_gctx : GoGlobalContext} : go.type := go.StructType [
+Definition Editor'fds_unsealed {ext : ffi_syntax} {go_gctx : GoGlobalContext} : list go.field_decl := [
   (go.FieldDecl "s"%go (go.SliceType go.uint64));
   (go.FieldDecl "next_val"%go go.uint64)
 ].
+Program Definition Editor'fds {ext : ffi_syntax} {go_gctx : GoGlobalContext} := sealed (Editor'fds_unsealed).
+Global Instance equals_unfold_Editor {ext : ffi_syntax} {go_gctx : GoGlobalContext} : Editor'fds =→ Editor'fds_unsealed.
+Proof. rewrite /Editor'fds seal_eq //. Qed.
+
+Definition Editorⁱᵐᵖˡ {ext : ffi_syntax} {go_gctx : GoGlobalContext} : go.type := go.StructType (Editor'fds).
 
 Class Editor_Assumptions {ext : ffi_syntax} `{!GoGlobalContext} `{!GoLocalContext} `{!GoSemanticsFunctions} : Prop :=
 {
-  #[global] Editor_type_repr  :: go.TypeRepr Editor Editor.t;
+  #[global] Editor_type_repr  :: go.TypeReprUnderlying Editorⁱᵐᵖˡ Editor.t;
   #[global] Editor_underlying :: (Editor) <u (Editorⁱᵐᵖˡ);
-  #[global] Editor_get_s (x : Editor.t) :: go.IsGoStepPureDet (StructFieldGet (Editor) "s") #x #x.(Editor.s');
-  #[global] Editor_set_s (x : Editor.t) y :: go.IsGoStepPureDet (StructFieldSet (Editor) "s") (#x, #y) #(x <|Editor.s' := y|>);
-  #[global] Editor_get_next_val (x : Editor.t) :: go.IsGoStepPureDet (StructFieldGet (Editor) "next_val") #x #x.(Editor.next_val');
-  #[global] Editor_set_next_val (x : Editor.t) y :: go.IsGoStepPureDet (StructFieldSet (Editor) "next_val") (#x, #y) #(x <|Editor.next_val' := y|>);
+  #[global] Editor_get_s (x : Editor.t) :: ⟦StructFieldGet (Editorⁱᵐᵖˡ) "s", #x⟧ ⤳[under] #x.(Editor.s');
+  #[global] Editor_set_s (x : Editor.t) y :: ⟦StructFieldSet (Editorⁱᵐᵖˡ) "s", (#x, #y)⟧ ⤳[under] #(x <|Editor.s' := y|>);
+  #[global] Editor_get_next_val (x : Editor.t) :: ⟦StructFieldGet (Editorⁱᵐᵖˡ) "next_val", #x⟧ ⤳[under] #x.(Editor.next_val');
+  #[global] Editor_set_next_val (x : Editor.t) y :: ⟦StructFieldSet (Editorⁱᵐᵖˡ) "next_val", (#x, #y)⟧ ⤳[under] #(x <|Editor.next_val' := y|>);
   #[global] Editor'ptr_AdvanceReturn_unfold :: MethodUnfold (go.PointerType (Editor)) "AdvanceReturn" (Editor__AdvanceReturnⁱᵐᵖˡ);
 }.
 
@@ -3110,19 +3131,24 @@ End def.
 
 End Pair.
 
-Definition Pairⁱᵐᵖˡ {ext : ffi_syntax} {go_gctx : GoGlobalContext} : go.type := go.StructType [
+Definition Pair'fds_unsealed {ext : ffi_syntax} {go_gctx : GoGlobalContext} : list go.field_decl := [
   (go.FieldDecl "x"%go go.uint64);
   (go.FieldDecl "y"%go go.uint64)
 ].
+Program Definition Pair'fds {ext : ffi_syntax} {go_gctx : GoGlobalContext} := sealed (Pair'fds_unsealed).
+Global Instance equals_unfold_Pair {ext : ffi_syntax} {go_gctx : GoGlobalContext} : Pair'fds =→ Pair'fds_unsealed.
+Proof. rewrite /Pair'fds seal_eq //. Qed.
+
+Definition Pairⁱᵐᵖˡ {ext : ffi_syntax} {go_gctx : GoGlobalContext} : go.type := go.StructType (Pair'fds).
 
 Class Pair_Assumptions {ext : ffi_syntax} `{!GoGlobalContext} `{!GoLocalContext} `{!GoSemanticsFunctions} : Prop :=
 {
-  #[global] Pair_type_repr  :: go.TypeRepr Pair Pair.t;
+  #[global] Pair_type_repr  :: go.TypeReprUnderlying Pairⁱᵐᵖˡ Pair.t;
   #[global] Pair_underlying :: (Pair) <u (Pairⁱᵐᵖˡ);
-  #[global] Pair_get_x (x : Pair.t) :: go.IsGoStepPureDet (StructFieldGet (Pair) "x") #x #x.(Pair.x');
-  #[global] Pair_set_x (x : Pair.t) y :: go.IsGoStepPureDet (StructFieldSet (Pair) "x") (#x, #y) #(x <|Pair.x' := y|>);
-  #[global] Pair_get_y (x : Pair.t) :: go.IsGoStepPureDet (StructFieldGet (Pair) "y") #x #x.(Pair.y');
-  #[global] Pair_set_y (x : Pair.t) y :: go.IsGoStepPureDet (StructFieldSet (Pair) "y") (#x, #y) #(x <|Pair.y' := y|>);
+  #[global] Pair_get_x (x : Pair.t) :: ⟦StructFieldGet (Pairⁱᵐᵖˡ) "x", #x⟧ ⤳[under] #x.(Pair.x');
+  #[global] Pair_set_x (x : Pair.t) y :: ⟦StructFieldSet (Pairⁱᵐᵖˡ) "x", (#x, #y)⟧ ⤳[under] #(x <|Pair.x' := y|>);
+  #[global] Pair_get_y (x : Pair.t) :: ⟦StructFieldGet (Pairⁱᵐᵖˡ) "y", #x⟧ ⤳[under] #x.(Pair.y');
+  #[global] Pair_set_y (x : Pair.t) y :: ⟦StructFieldSet (Pairⁱᵐᵖˡ) "y", (#x, #y)⟧ ⤳[under] #(x <|Pair.y' := y|>);
 }.
 
 Module Uint32.
@@ -3136,7 +3162,6 @@ Definition Uint32ⁱᵐᵖˡ {ext : ffi_syntax} {go_gctx : GoGlobalContext} : go
 
 Class Uint32_Assumptions {ext : ffi_syntax} `{!GoGlobalContext} `{!GoLocalContext} `{!GoSemanticsFunctions} : Prop :=
 {
-  #[global] Uint32_type_repr  :: go.TypeRepr Uint32 Uint32.t;
   #[global] Uint32_underlying :: (Uint32) <u (Uint32ⁱᵐᵖˡ);
 }.
 
@@ -3151,7 +3176,6 @@ Definition geometryInterfaceⁱᵐᵖˡ {ext : ffi_syntax} {go_gctx : GoGlobalCo
 
 Class geometryInterface_Assumptions {ext : ffi_syntax} `{!GoGlobalContext} `{!GoLocalContext} `{!GoSemanticsFunctions} : Prop :=
 {
-  #[global] geometryInterface_type_repr  :: go.TypeRepr geometryInterface geometryInterface.t;
   #[global] geometryInterface_underlying :: (geometryInterface) <u (geometryInterfaceⁱᵐᵖˡ);
 }.
 
@@ -3170,16 +3194,21 @@ End def.
 
 End SquareStruct.
 
-Definition SquareStructⁱᵐᵖˡ {ext : ffi_syntax} {go_gctx : GoGlobalContext} : go.type := go.StructType [
+Definition SquareStruct'fds_unsealed {ext : ffi_syntax} {go_gctx : GoGlobalContext} : list go.field_decl := [
   (go.FieldDecl "Side"%go go.uint64)
 ].
+Program Definition SquareStruct'fds {ext : ffi_syntax} {go_gctx : GoGlobalContext} := sealed (SquareStruct'fds_unsealed).
+Global Instance equals_unfold_SquareStruct {ext : ffi_syntax} {go_gctx : GoGlobalContext} : SquareStruct'fds =→ SquareStruct'fds_unsealed.
+Proof. rewrite /SquareStruct'fds seal_eq //. Qed.
+
+Definition SquareStructⁱᵐᵖˡ {ext : ffi_syntax} {go_gctx : GoGlobalContext} : go.type := go.StructType (SquareStruct'fds).
 
 Class SquareStruct_Assumptions {ext : ffi_syntax} `{!GoGlobalContext} `{!GoLocalContext} `{!GoSemanticsFunctions} : Prop :=
 {
-  #[global] SquareStruct_type_repr  :: go.TypeRepr SquareStruct SquareStruct.t;
+  #[global] SquareStruct_type_repr  :: go.TypeReprUnderlying SquareStructⁱᵐᵖˡ SquareStruct.t;
   #[global] SquareStruct_underlying :: (SquareStruct) <u (SquareStructⁱᵐᵖˡ);
-  #[global] SquareStruct_get_Side (x : SquareStruct.t) :: go.IsGoStepPureDet (StructFieldGet (SquareStruct) "Side") #x #x.(SquareStruct.Side');
-  #[global] SquareStruct_set_Side (x : SquareStruct.t) y :: go.IsGoStepPureDet (StructFieldSet (SquareStruct) "Side") (#x, #y) #(x <|SquareStruct.Side' := y|>);
+  #[global] SquareStruct_get_Side (x : SquareStruct.t) :: ⟦StructFieldGet (SquareStructⁱᵐᵖˡ) "Side", #x⟧ ⤳[under] #x.(SquareStruct.Side');
+  #[global] SquareStruct_set_Side (x : SquareStruct.t) y :: ⟦StructFieldSet (SquareStructⁱᵐᵖˡ) "Side", (#x, #y)⟧ ⤳[under] #(x <|SquareStruct.Side' := y|>);
   #[global] SquareStruct_Square_unfold :: MethodUnfold (SquareStruct) "Square" (SquareStruct__Squareⁱᵐᵖˡ);
   #[global] SquareStruct_Volume_unfold :: MethodUnfold (SquareStruct) "Volume" (SquareStruct__Volumeⁱᵐᵖˡ);
   #[global] SquareStruct'ptr_Square_unfold :: MethodUnfold (go.PointerType (SquareStruct)) "Square" (λ: "$r", MethodResolve (SquareStruct) "Square" (![(SquareStruct)] "$r"));
@@ -3201,16 +3230,21 @@ End def.
 
 End LoopStruct.
 
-Definition LoopStructⁱᵐᵖˡ {ext : ffi_syntax} {go_gctx : GoGlobalContext} : go.type := go.StructType [
+Definition LoopStruct'fds_unsealed {ext : ffi_syntax} {go_gctx : GoGlobalContext} : list go.field_decl := [
   (go.FieldDecl "loopNext"%go (go.PointerType go.uint64))
 ].
+Program Definition LoopStruct'fds {ext : ffi_syntax} {go_gctx : GoGlobalContext} := sealed (LoopStruct'fds_unsealed).
+Global Instance equals_unfold_LoopStruct {ext : ffi_syntax} {go_gctx : GoGlobalContext} : LoopStruct'fds =→ LoopStruct'fds_unsealed.
+Proof. rewrite /LoopStruct'fds seal_eq //. Qed.
+
+Definition LoopStructⁱᵐᵖˡ {ext : ffi_syntax} {go_gctx : GoGlobalContext} : go.type := go.StructType (LoopStruct'fds).
 
 Class LoopStruct_Assumptions {ext : ffi_syntax} `{!GoGlobalContext} `{!GoLocalContext} `{!GoSemanticsFunctions} : Prop :=
 {
-  #[global] LoopStruct_type_repr  :: go.TypeRepr LoopStruct LoopStruct.t;
+  #[global] LoopStruct_type_repr  :: go.TypeReprUnderlying LoopStructⁱᵐᵖˡ LoopStruct.t;
   #[global] LoopStruct_underlying :: (LoopStruct) <u (LoopStructⁱᵐᵖˡ);
-  #[global] LoopStruct_get_loopNext (x : LoopStruct.t) :: go.IsGoStepPureDet (StructFieldGet (LoopStruct) "loopNext") #x #x.(LoopStruct.loopNext');
-  #[global] LoopStruct_set_loopNext (x : LoopStruct.t) y :: go.IsGoStepPureDet (StructFieldSet (LoopStruct) "loopNext") (#x, #y) #(x <|LoopStruct.loopNext' := y|>);
+  #[global] LoopStruct_get_loopNext (x : LoopStruct.t) :: ⟦StructFieldGet (LoopStructⁱᵐᵖˡ) "loopNext", #x⟧ ⤳[under] #x.(LoopStruct.loopNext');
+  #[global] LoopStruct_set_loopNext (x : LoopStruct.t) y :: ⟦StructFieldSet (LoopStructⁱᵐᵖˡ) "loopNext", (#x, #y)⟧ ⤳[under] #(x <|LoopStruct.loopNext' := y|>);
   #[global] LoopStruct_forLoopWait_unfold :: MethodUnfold (LoopStruct) "forLoopWait" (LoopStruct__forLoopWaitⁱᵐᵖˡ);
   #[global] LoopStruct'ptr_forLoopWait_unfold :: MethodUnfold (go.PointerType (LoopStruct)) "forLoopWait" (λ: "$r", MethodResolve (LoopStruct) "forLoopWait" (![(LoopStruct)] "$r"));
 }.
@@ -3233,25 +3267,30 @@ End def.
 
 End BoolTest.
 
-Definition BoolTestⁱᵐᵖˡ {ext : ffi_syntax} {go_gctx : GoGlobalContext} : go.type := go.StructType [
+Definition BoolTest'fds_unsealed {ext : ffi_syntax} {go_gctx : GoGlobalContext} : list go.field_decl := [
   (go.FieldDecl "t"%go go.bool);
   (go.FieldDecl "f"%go go.bool);
   (go.FieldDecl "tc"%go go.uint64);
   (go.FieldDecl "fc"%go go.uint64)
 ].
+Program Definition BoolTest'fds {ext : ffi_syntax} {go_gctx : GoGlobalContext} := sealed (BoolTest'fds_unsealed).
+Global Instance equals_unfold_BoolTest {ext : ffi_syntax} {go_gctx : GoGlobalContext} : BoolTest'fds =→ BoolTest'fds_unsealed.
+Proof. rewrite /BoolTest'fds seal_eq //. Qed.
+
+Definition BoolTestⁱᵐᵖˡ {ext : ffi_syntax} {go_gctx : GoGlobalContext} : go.type := go.StructType (BoolTest'fds).
 
 Class BoolTest_Assumptions {ext : ffi_syntax} `{!GoGlobalContext} `{!GoLocalContext} `{!GoSemanticsFunctions} : Prop :=
 {
-  #[global] BoolTest_type_repr  :: go.TypeRepr BoolTest BoolTest.t;
+  #[global] BoolTest_type_repr  :: go.TypeReprUnderlying BoolTestⁱᵐᵖˡ BoolTest.t;
   #[global] BoolTest_underlying :: (BoolTest) <u (BoolTestⁱᵐᵖˡ);
-  #[global] BoolTest_get_t (x : BoolTest.t) :: go.IsGoStepPureDet (StructFieldGet (BoolTest) "t") #x #x.(BoolTest.t');
-  #[global] BoolTest_set_t (x : BoolTest.t) y :: go.IsGoStepPureDet (StructFieldSet (BoolTest) "t") (#x, #y) #(x <|BoolTest.t' := y|>);
-  #[global] BoolTest_get_f (x : BoolTest.t) :: go.IsGoStepPureDet (StructFieldGet (BoolTest) "f") #x #x.(BoolTest.f');
-  #[global] BoolTest_set_f (x : BoolTest.t) y :: go.IsGoStepPureDet (StructFieldSet (BoolTest) "f") (#x, #y) #(x <|BoolTest.f' := y|>);
-  #[global] BoolTest_get_tc (x : BoolTest.t) :: go.IsGoStepPureDet (StructFieldGet (BoolTest) "tc") #x #x.(BoolTest.tc');
-  #[global] BoolTest_set_tc (x : BoolTest.t) y :: go.IsGoStepPureDet (StructFieldSet (BoolTest) "tc") (#x, #y) #(x <|BoolTest.tc' := y|>);
-  #[global] BoolTest_get_fc (x : BoolTest.t) :: go.IsGoStepPureDet (StructFieldGet (BoolTest) "fc") #x #x.(BoolTest.fc');
-  #[global] BoolTest_set_fc (x : BoolTest.t) y :: go.IsGoStepPureDet (StructFieldSet (BoolTest) "fc") (#x, #y) #(x <|BoolTest.fc' := y|>);
+  #[global] BoolTest_get_t (x : BoolTest.t) :: ⟦StructFieldGet (BoolTestⁱᵐᵖˡ) "t", #x⟧ ⤳[under] #x.(BoolTest.t');
+  #[global] BoolTest_set_t (x : BoolTest.t) y :: ⟦StructFieldSet (BoolTestⁱᵐᵖˡ) "t", (#x, #y)⟧ ⤳[under] #(x <|BoolTest.t' := y|>);
+  #[global] BoolTest_get_f (x : BoolTest.t) :: ⟦StructFieldGet (BoolTestⁱᵐᵖˡ) "f", #x⟧ ⤳[under] #x.(BoolTest.f');
+  #[global] BoolTest_set_f (x : BoolTest.t) y :: ⟦StructFieldSet (BoolTestⁱᵐᵖˡ) "f", (#x, #y)⟧ ⤳[under] #(x <|BoolTest.f' := y|>);
+  #[global] BoolTest_get_tc (x : BoolTest.t) :: ⟦StructFieldGet (BoolTestⁱᵐᵖˡ) "tc", #x⟧ ⤳[under] #x.(BoolTest.tc');
+  #[global] BoolTest_set_tc (x : BoolTest.t) y :: ⟦StructFieldSet (BoolTestⁱᵐᵖˡ) "tc", (#x, #y)⟧ ⤳[under] #(x <|BoolTest.tc' := y|>);
+  #[global] BoolTest_get_fc (x : BoolTest.t) :: ⟦StructFieldGet (BoolTestⁱᵐᵖˡ) "fc", #x⟧ ⤳[under] #x.(BoolTest.fc');
+  #[global] BoolTest_set_fc (x : BoolTest.t) y :: ⟦StructFieldSet (BoolTestⁱᵐᵖˡ) "fc", (#x, #y)⟧ ⤳[under] #(x <|BoolTest.fc' := y|>);
 }.
 
 Module ArrayEditor.
@@ -3270,19 +3309,24 @@ End def.
 
 End ArrayEditor.
 
-Definition ArrayEditorⁱᵐᵖˡ {ext : ffi_syntax} {go_gctx : GoGlobalContext} : go.type := go.StructType [
+Definition ArrayEditor'fds_unsealed {ext : ffi_syntax} {go_gctx : GoGlobalContext} : list go.field_decl := [
   (go.FieldDecl "s"%go (go.SliceType go.uint64));
   (go.FieldDecl "next_val"%go go.uint64)
 ].
+Program Definition ArrayEditor'fds {ext : ffi_syntax} {go_gctx : GoGlobalContext} := sealed (ArrayEditor'fds_unsealed).
+Global Instance equals_unfold_ArrayEditor {ext : ffi_syntax} {go_gctx : GoGlobalContext} : ArrayEditor'fds =→ ArrayEditor'fds_unsealed.
+Proof. rewrite /ArrayEditor'fds seal_eq //. Qed.
+
+Definition ArrayEditorⁱᵐᵖˡ {ext : ffi_syntax} {go_gctx : GoGlobalContext} : go.type := go.StructType (ArrayEditor'fds).
 
 Class ArrayEditor_Assumptions {ext : ffi_syntax} `{!GoGlobalContext} `{!GoLocalContext} `{!GoSemanticsFunctions} : Prop :=
 {
-  #[global] ArrayEditor_type_repr  :: go.TypeRepr ArrayEditor ArrayEditor.t;
+  #[global] ArrayEditor_type_repr  :: go.TypeReprUnderlying ArrayEditorⁱᵐᵖˡ ArrayEditor.t;
   #[global] ArrayEditor_underlying :: (ArrayEditor) <u (ArrayEditorⁱᵐᵖˡ);
-  #[global] ArrayEditor_get_s (x : ArrayEditor.t) :: go.IsGoStepPureDet (StructFieldGet (ArrayEditor) "s") #x #x.(ArrayEditor.s');
-  #[global] ArrayEditor_set_s (x : ArrayEditor.t) y :: go.IsGoStepPureDet (StructFieldSet (ArrayEditor) "s") (#x, #y) #(x <|ArrayEditor.s' := y|>);
-  #[global] ArrayEditor_get_next_val (x : ArrayEditor.t) :: go.IsGoStepPureDet (StructFieldGet (ArrayEditor) "next_val") #x #x.(ArrayEditor.next_val');
-  #[global] ArrayEditor_set_next_val (x : ArrayEditor.t) y :: go.IsGoStepPureDet (StructFieldSet (ArrayEditor) "next_val") (#x, #y) #(x <|ArrayEditor.next_val' := y|>);
+  #[global] ArrayEditor_get_s (x : ArrayEditor.t) :: ⟦StructFieldGet (ArrayEditorⁱᵐᵖˡ) "s", #x⟧ ⤳[under] #x.(ArrayEditor.s');
+  #[global] ArrayEditor_set_s (x : ArrayEditor.t) y :: ⟦StructFieldSet (ArrayEditorⁱᵐᵖˡ) "s", (#x, #y)⟧ ⤳[under] #(x <|ArrayEditor.s' := y|>);
+  #[global] ArrayEditor_get_next_val (x : ArrayEditor.t) :: ⟦StructFieldGet (ArrayEditorⁱᵐᵖˡ) "next_val", #x⟧ ⤳[under] #x.(ArrayEditor.next_val');
+  #[global] ArrayEditor_set_next_val (x : ArrayEditor.t) y :: ⟦StructFieldSet (ArrayEditorⁱᵐᵖˡ) "next_val", (#x, #y)⟧ ⤳[under] #(x <|ArrayEditor.next_val' := y|>);
   #[global] ArrayEditor'ptr_Advance_unfold :: MethodUnfold (go.PointerType (ArrayEditor)) "Advance" (ArrayEditor__Advanceⁱᵐᵖˡ);
 }.
 
@@ -3302,19 +3346,24 @@ End def.
 
 End Bar.
 
-Definition Barⁱᵐᵖˡ {ext : ffi_syntax} {go_gctx : GoGlobalContext} : go.type := go.StructType [
+Definition Bar'fds_unsealed {ext : ffi_syntax} {go_gctx : GoGlobalContext} : list go.field_decl := [
   (go.FieldDecl "a"%go go.uint64);
   (go.FieldDecl "b"%go go.uint64)
 ].
+Program Definition Bar'fds {ext : ffi_syntax} {go_gctx : GoGlobalContext} := sealed (Bar'fds_unsealed).
+Global Instance equals_unfold_Bar {ext : ffi_syntax} {go_gctx : GoGlobalContext} : Bar'fds =→ Bar'fds_unsealed.
+Proof. rewrite /Bar'fds seal_eq //. Qed.
+
+Definition Barⁱᵐᵖˡ {ext : ffi_syntax} {go_gctx : GoGlobalContext} : go.type := go.StructType (Bar'fds).
 
 Class Bar_Assumptions {ext : ffi_syntax} `{!GoGlobalContext} `{!GoLocalContext} `{!GoSemanticsFunctions} : Prop :=
 {
-  #[global] Bar_type_repr  :: go.TypeRepr Bar Bar.t;
+  #[global] Bar_type_repr  :: go.TypeReprUnderlying Barⁱᵐᵖˡ Bar.t;
   #[global] Bar_underlying :: (Bar) <u (Barⁱᵐᵖˡ);
-  #[global] Bar_get_a (x : Bar.t) :: go.IsGoStepPureDet (StructFieldGet (Bar) "a") #x #x.(Bar.a');
-  #[global] Bar_set_a (x : Bar.t) y :: go.IsGoStepPureDet (StructFieldSet (Bar) "a") (#x, #y) #(x <|Bar.a' := y|>);
-  #[global] Bar_get_b (x : Bar.t) :: go.IsGoStepPureDet (StructFieldGet (Bar) "b") #x #x.(Bar.b');
-  #[global] Bar_set_b (x : Bar.t) y :: go.IsGoStepPureDet (StructFieldSet (Bar) "b") (#x, #y) #(x <|Bar.b' := y|>);
+  #[global] Bar_get_a (x : Bar.t) :: ⟦StructFieldGet (Barⁱᵐᵖˡ) "a", #x⟧ ⤳[under] #x.(Bar.a');
+  #[global] Bar_set_a (x : Bar.t) y :: ⟦StructFieldSet (Barⁱᵐᵖˡ) "a", (#x, #y)⟧ ⤳[under] #(x <|Bar.a' := y|>);
+  #[global] Bar_get_b (x : Bar.t) :: ⟦StructFieldGet (Barⁱᵐᵖˡ) "b", #x⟧ ⤳[under] #x.(Bar.b');
+  #[global] Bar_set_b (x : Bar.t) y :: ⟦StructFieldSet (Barⁱᵐᵖˡ) "b", (#x, #y)⟧ ⤳[under] #(x <|Bar.b' := y|>);
   #[global] Bar'ptr_mutate_unfold :: MethodUnfold (go.PointerType (Bar)) "mutate" (Bar__mutateⁱᵐᵖˡ);
 }.
 
@@ -3333,16 +3382,21 @@ End def.
 
 End Foo.
 
-Definition Fooⁱᵐᵖˡ {ext : ffi_syntax} {go_gctx : GoGlobalContext} : go.type := go.StructType [
+Definition Foo'fds_unsealed {ext : ffi_syntax} {go_gctx : GoGlobalContext} : list go.field_decl := [
   (go.FieldDecl "bar"%go Bar)
 ].
+Program Definition Foo'fds {ext : ffi_syntax} {go_gctx : GoGlobalContext} := sealed (Foo'fds_unsealed).
+Global Instance equals_unfold_Foo {ext : ffi_syntax} {go_gctx : GoGlobalContext} : Foo'fds =→ Foo'fds_unsealed.
+Proof. rewrite /Foo'fds seal_eq //. Qed.
+
+Definition Fooⁱᵐᵖˡ {ext : ffi_syntax} {go_gctx : GoGlobalContext} : go.type := go.StructType (Foo'fds).
 
 Class Foo_Assumptions {ext : ffi_syntax} `{!GoGlobalContext} `{!GoLocalContext} `{!GoSemanticsFunctions} : Prop :=
 {
-  #[global] Foo_type_repr  :: go.TypeRepr Foo Foo.t;
+  #[global] Foo_type_repr  :: go.TypeReprUnderlying Fooⁱᵐᵖˡ Foo.t;
   #[global] Foo_underlying :: (Foo) <u (Fooⁱᵐᵖˡ);
-  #[global] Foo_get_bar (x : Foo.t) :: go.IsGoStepPureDet (StructFieldGet (Foo) "bar") #x #x.(Foo.bar');
-  #[global] Foo_set_bar (x : Foo.t) y :: go.IsGoStepPureDet (StructFieldSet (Foo) "bar") (#x, #y) #(x <|Foo.bar' := y|>);
+  #[global] Foo_get_bar (x : Foo.t) :: ⟦StructFieldGet (Fooⁱᵐᵖˡ) "bar", #x⟧ ⤳[under] #x.(Foo.bar');
+  #[global] Foo_set_bar (x : Foo.t) y :: ⟦StructFieldSet (Fooⁱᵐᵖˡ) "bar", (#x, #y)⟧ ⤳[under] #(x <|Foo.bar' := y|>);
   #[global] Foo'ptr_mutateBar_unfold :: MethodUnfold (go.PointerType (Foo)) "mutateBar" (Foo__mutateBarⁱᵐᵖˡ);
 }.
 
@@ -3362,19 +3416,24 @@ End def.
 
 End TwoInts.
 
-Definition TwoIntsⁱᵐᵖˡ {ext : ffi_syntax} {go_gctx : GoGlobalContext} : go.type := go.StructType [
+Definition TwoInts'fds_unsealed {ext : ffi_syntax} {go_gctx : GoGlobalContext} : list go.field_decl := [
   (go.FieldDecl "x"%go go.uint64);
   (go.FieldDecl "y"%go go.uint64)
 ].
+Program Definition TwoInts'fds {ext : ffi_syntax} {go_gctx : GoGlobalContext} := sealed (TwoInts'fds_unsealed).
+Global Instance equals_unfold_TwoInts {ext : ffi_syntax} {go_gctx : GoGlobalContext} : TwoInts'fds =→ TwoInts'fds_unsealed.
+Proof. rewrite /TwoInts'fds seal_eq //. Qed.
+
+Definition TwoIntsⁱᵐᵖˡ {ext : ffi_syntax} {go_gctx : GoGlobalContext} : go.type := go.StructType (TwoInts'fds).
 
 Class TwoInts_Assumptions {ext : ffi_syntax} `{!GoGlobalContext} `{!GoLocalContext} `{!GoSemanticsFunctions} : Prop :=
 {
-  #[global] TwoInts_type_repr  :: go.TypeRepr TwoInts TwoInts.t;
+  #[global] TwoInts_type_repr  :: go.TypeReprUnderlying TwoIntsⁱᵐᵖˡ TwoInts.t;
   #[global] TwoInts_underlying :: (TwoInts) <u (TwoIntsⁱᵐᵖˡ);
-  #[global] TwoInts_get_x (x : TwoInts.t) :: go.IsGoStepPureDet (StructFieldGet (TwoInts) "x") #x #x.(TwoInts.x');
-  #[global] TwoInts_set_x (x : TwoInts.t) y :: go.IsGoStepPureDet (StructFieldSet (TwoInts) "x") (#x, #y) #(x <|TwoInts.x' := y|>);
-  #[global] TwoInts_get_y (x : TwoInts.t) :: go.IsGoStepPureDet (StructFieldGet (TwoInts) "y") #x #x.(TwoInts.y');
-  #[global] TwoInts_set_y (x : TwoInts.t) y :: go.IsGoStepPureDet (StructFieldSet (TwoInts) "y") (#x, #y) #(x <|TwoInts.y' := y|>);
+  #[global] TwoInts_get_x (x : TwoInts.t) :: ⟦StructFieldGet (TwoIntsⁱᵐᵖˡ) "x", #x⟧ ⤳[under] #x.(TwoInts.x');
+  #[global] TwoInts_set_x (x : TwoInts.t) y :: ⟦StructFieldSet (TwoIntsⁱᵐᵖˡ) "x", (#x, #y)⟧ ⤳[under] #(x <|TwoInts.x' := y|>);
+  #[global] TwoInts_get_y (x : TwoInts.t) :: ⟦StructFieldGet (TwoIntsⁱᵐᵖˡ) "y", #x⟧ ⤳[under] #x.(TwoInts.y');
+  #[global] TwoInts_set_y (x : TwoInts.t) y :: ⟦StructFieldSet (TwoIntsⁱᵐᵖˡ) "y", (#x, #y)⟧ ⤳[under] #(x <|TwoInts.y' := y|>);
 }.
 
 Module S.
@@ -3394,22 +3453,27 @@ End def.
 
 End S.
 
-Definition Sⁱᵐᵖˡ {ext : ffi_syntax} {go_gctx : GoGlobalContext} : go.type := go.StructType [
+Definition S'fds_unsealed {ext : ffi_syntax} {go_gctx : GoGlobalContext} : list go.field_decl := [
   (go.FieldDecl "a"%go go.uint64);
   (go.FieldDecl "b"%go TwoInts);
   (go.FieldDecl "c"%go go.bool)
 ].
+Program Definition S'fds {ext : ffi_syntax} {go_gctx : GoGlobalContext} := sealed (S'fds_unsealed).
+Global Instance equals_unfold_S {ext : ffi_syntax} {go_gctx : GoGlobalContext} : S'fds =→ S'fds_unsealed.
+Proof. rewrite /S'fds seal_eq //. Qed.
+
+Definition Sⁱᵐᵖˡ {ext : ffi_syntax} {go_gctx : GoGlobalContext} : go.type := go.StructType (S'fds).
 
 Class S_Assumptions {ext : ffi_syntax} `{!GoGlobalContext} `{!GoLocalContext} `{!GoSemanticsFunctions} : Prop :=
 {
-  #[global] S_type_repr  :: go.TypeRepr S S.t;
+  #[global] S_type_repr  :: go.TypeReprUnderlying Sⁱᵐᵖˡ S.t;
   #[global] S_underlying :: (S) <u (Sⁱᵐᵖˡ);
-  #[global] S_get_a (x : S.t) :: go.IsGoStepPureDet (StructFieldGet (S) "a") #x #x.(S.a');
-  #[global] S_set_a (x : S.t) y :: go.IsGoStepPureDet (StructFieldSet (S) "a") (#x, #y) #(x <|S.a' := y|>);
-  #[global] S_get_b (x : S.t) :: go.IsGoStepPureDet (StructFieldGet (S) "b") #x #x.(S.b');
-  #[global] S_set_b (x : S.t) y :: go.IsGoStepPureDet (StructFieldSet (S) "b") (#x, #y) #(x <|S.b' := y|>);
-  #[global] S_get_c (x : S.t) :: go.IsGoStepPureDet (StructFieldGet (S) "c") #x #x.(S.c');
-  #[global] S_set_c (x : S.t) y :: go.IsGoStepPureDet (StructFieldSet (S) "c") (#x, #y) #(x <|S.c' := y|>);
+  #[global] S_get_a (x : S.t) :: ⟦StructFieldGet (Sⁱᵐᵖˡ) "a", #x⟧ ⤳[under] #x.(S.a');
+  #[global] S_set_a (x : S.t) y :: ⟦StructFieldSet (Sⁱᵐᵖˡ) "a", (#x, #y)⟧ ⤳[under] #(x <|S.a' := y|>);
+  #[global] S_get_b (x : S.t) :: ⟦StructFieldGet (Sⁱᵐᵖˡ) "b", #x⟧ ⤳[under] #x.(S.b');
+  #[global] S_set_b (x : S.t) y :: ⟦StructFieldSet (Sⁱᵐᵖˡ) "b", (#x, #y)⟧ ⤳[under] #(x <|S.b' := y|>);
+  #[global] S_get_c (x : S.t) :: ⟦StructFieldGet (Sⁱᵐᵖˡ) "c", #x⟧ ⤳[under] #x.(S.c');
+  #[global] S_set_c (x : S.t) y :: ⟦StructFieldSet (Sⁱᵐᵖˡ) "c", (#x, #y)⟧ ⤳[under] #(x <|S.c' := y|>);
   #[global] S_readBVal_unfold :: MethodUnfold (S) "readBVal" (S__readBValⁱᵐᵖˡ);
   #[global] S'ptr_negateC_unfold :: MethodUnfold (go.PointerType (S)) "negateC" (S__negateCⁱᵐᵖˡ);
   #[global] S'ptr_readA_unfold :: MethodUnfold (go.PointerType (S)) "readA" (S__readAⁱᵐᵖˡ);
@@ -3433,16 +3497,21 @@ End def.
 
 End StructWrap.
 
-Definition StructWrapⁱᵐᵖˡ {ext : ffi_syntax} {go_gctx : GoGlobalContext} : go.type := go.StructType [
+Definition StructWrap'fds_unsealed {ext : ffi_syntax} {go_gctx : GoGlobalContext} : list go.field_decl := [
   (go.FieldDecl "i"%go go.uint64)
 ].
+Program Definition StructWrap'fds {ext : ffi_syntax} {go_gctx : GoGlobalContext} := sealed (StructWrap'fds_unsealed).
+Global Instance equals_unfold_StructWrap {ext : ffi_syntax} {go_gctx : GoGlobalContext} : StructWrap'fds =→ StructWrap'fds_unsealed.
+Proof. rewrite /StructWrap'fds seal_eq //. Qed.
+
+Definition StructWrapⁱᵐᵖˡ {ext : ffi_syntax} {go_gctx : GoGlobalContext} : go.type := go.StructType (StructWrap'fds).
 
 Class StructWrap_Assumptions {ext : ffi_syntax} `{!GoGlobalContext} `{!GoLocalContext} `{!GoSemanticsFunctions} : Prop :=
 {
-  #[global] StructWrap_type_repr  :: go.TypeRepr StructWrap StructWrap.t;
+  #[global] StructWrap_type_repr  :: go.TypeReprUnderlying StructWrapⁱᵐᵖˡ StructWrap.t;
   #[global] StructWrap_underlying :: (StructWrap) <u (StructWrapⁱᵐᵖˡ);
-  #[global] StructWrap_get_i (x : StructWrap.t) :: go.IsGoStepPureDet (StructFieldGet (StructWrap) "i") #x #x.(StructWrap.i');
-  #[global] StructWrap_set_i (x : StructWrap.t) y :: go.IsGoStepPureDet (StructFieldSet (StructWrap) "i") (#x, #y) #(x <|StructWrap.i' := y|>);
+  #[global] StructWrap_get_i (x : StructWrap.t) :: ⟦StructFieldGet (StructWrapⁱᵐᵖˡ) "i", #x⟧ ⤳[under] #x.(StructWrap.i');
+  #[global] StructWrap_set_i (x : StructWrap.t) y :: ⟦StructFieldSet (StructWrapⁱᵐᵖˡ) "i", (#x, #y)⟧ ⤳[under] #(x <|StructWrap.i' := y|>);
 }.
 
 Module StructWithFunc.
@@ -3460,16 +3529,21 @@ End def.
 
 End StructWithFunc.
 
-Definition StructWithFuncⁱᵐᵖˡ {ext : ffi_syntax} {go_gctx : GoGlobalContext} : go.type := go.StructType [
+Definition StructWithFunc'fds_unsealed {ext : ffi_syntax} {go_gctx : GoGlobalContext} : list go.field_decl := [
   (go.FieldDecl "fn"%go (go.FunctionType (go.Signature [go.uint64] false [go.uint64])))
 ].
+Program Definition StructWithFunc'fds {ext : ffi_syntax} {go_gctx : GoGlobalContext} := sealed (StructWithFunc'fds_unsealed).
+Global Instance equals_unfold_StructWithFunc {ext : ffi_syntax} {go_gctx : GoGlobalContext} : StructWithFunc'fds =→ StructWithFunc'fds_unsealed.
+Proof. rewrite /StructWithFunc'fds seal_eq //. Qed.
+
+Definition StructWithFuncⁱᵐᵖˡ {ext : ffi_syntax} {go_gctx : GoGlobalContext} : go.type := go.StructType (StructWithFunc'fds).
 
 Class StructWithFunc_Assumptions {ext : ffi_syntax} `{!GoGlobalContext} `{!GoLocalContext} `{!GoSemanticsFunctions} : Prop :=
 {
-  #[global] StructWithFunc_type_repr  :: go.TypeRepr StructWithFunc StructWithFunc.t;
+  #[global] StructWithFunc_type_repr  :: go.TypeReprUnderlying StructWithFuncⁱᵐᵖˡ StructWithFunc.t;
   #[global] StructWithFunc_underlying :: (StructWithFunc) <u (StructWithFuncⁱᵐᵖˡ);
-  #[global] StructWithFunc_get_fn (x : StructWithFunc.t) :: go.IsGoStepPureDet (StructFieldGet (StructWithFunc) "fn") #x #x.(StructWithFunc.fn');
-  #[global] StructWithFunc_set_fn (x : StructWithFunc.t) y :: go.IsGoStepPureDet (StructFieldSet (StructWithFunc) "fn") (#x, #y) #(x <|StructWithFunc.fn' := y|>);
+  #[global] StructWithFunc_get_fn (x : StructWithFunc.t) :: ⟦StructFieldGet (StructWithFuncⁱᵐᵖˡ) "fn", #x⟧ ⤳[under] #x.(StructWithFunc.fn');
+  #[global] StructWithFunc_set_fn (x : StructWithFunc.t) y :: ⟦StructFieldSet (StructWithFuncⁱᵐᵖˡ) "fn", (#x, #y)⟧ ⤳[under] #(x <|StructWithFunc.fn' := y|>);
 }.
 
 Module switchConcrete.
@@ -3486,12 +3560,18 @@ End def.
 
 End switchConcrete.
 
-Definition switchConcreteⁱᵐᵖˡ {ext : ffi_syntax} {go_gctx : GoGlobalContext} : go.type := go.StructType [
+Definition switchConcrete'fds_unsealed {ext : ffi_syntax} {go_gctx : GoGlobalContext} : list go.field_decl := [
+
 ].
+Program Definition switchConcrete'fds {ext : ffi_syntax} {go_gctx : GoGlobalContext} := sealed (switchConcrete'fds_unsealed).
+Global Instance equals_unfold_switchConcrete {ext : ffi_syntax} {go_gctx : GoGlobalContext} : switchConcrete'fds =→ switchConcrete'fds_unsealed.
+Proof. rewrite /switchConcrete'fds seal_eq //. Qed.
+
+Definition switchConcreteⁱᵐᵖˡ {ext : ffi_syntax} {go_gctx : GoGlobalContext} : go.type := go.StructType (switchConcrete'fds).
 
 Class switchConcrete_Assumptions {ext : ffi_syntax} `{!GoGlobalContext} `{!GoLocalContext} `{!GoSemanticsFunctions} : Prop :=
 {
-  #[global] switchConcrete_type_repr  :: go.TypeRepr switchConcrete switchConcrete.t;
+  #[global] switchConcrete_type_repr  :: go.TypeReprUnderlying switchConcreteⁱᵐᵖˡ switchConcrete.t;
   #[global] switchConcrete_underlying :: (switchConcrete) <u (switchConcreteⁱᵐᵖˡ);
   #[global] switchConcrete'ptr_marker_unfold :: MethodUnfold (go.PointerType (switchConcrete)) "marker" (switchConcrete__markerⁱᵐᵖˡ);
 }.
@@ -3507,7 +3587,6 @@ Definition switchInterfaceⁱᵐᵖˡ {ext : ffi_syntax} {go_gctx : GoGlobalCont
 
 Class switchInterface_Assumptions {ext : ffi_syntax} `{!GoGlobalContext} `{!GoLocalContext} `{!GoSemanticsFunctions} : Prop :=
 {
-  #[global] switchInterface_type_repr  :: go.TypeRepr switchInterface switchInterface.t;
   #[global] switchInterface_underlying :: (switchInterface) <u (switchInterfaceⁱᵐᵖˡ);
 }.
 
@@ -3529,25 +3608,30 @@ End def.
 
 End Log.
 
-Definition Logⁱᵐᵖˡ {ext : ffi_syntax} {go_gctx : GoGlobalContext} : go.type := go.StructType [
+Definition Log'fds_unsealed {ext : ffi_syntax} {go_gctx : GoGlobalContext} : list go.field_decl := [
   (go.FieldDecl "d"%go disk.Disk);
   (go.FieldDecl "l"%go (go.PointerType sync.Mutex));
   (go.FieldDecl "cache"%go (go.MapType go.uint64 disk.Block));
   (go.FieldDecl "length"%go (go.PointerType go.uint64))
 ].
+Program Definition Log'fds {ext : ffi_syntax} {go_gctx : GoGlobalContext} := sealed (Log'fds_unsealed).
+Global Instance equals_unfold_Log {ext : ffi_syntax} {go_gctx : GoGlobalContext} : Log'fds =→ Log'fds_unsealed.
+Proof. rewrite /Log'fds seal_eq //. Qed.
+
+Definition Logⁱᵐᵖˡ {ext : ffi_syntax} {go_gctx : GoGlobalContext} : go.type := go.StructType (Log'fds).
 
 Class Log_Assumptions {ext : ffi_syntax} `{!GoGlobalContext} `{!GoLocalContext} `{!GoSemanticsFunctions} : Prop :=
 {
-  #[global] Log_type_repr  :: go.TypeRepr Log Log.t;
+  #[global] Log_type_repr  :: go.TypeReprUnderlying Logⁱᵐᵖˡ Log.t;
   #[global] Log_underlying :: (Log) <u (Logⁱᵐᵖˡ);
-  #[global] Log_get_d (x : Log.t) :: go.IsGoStepPureDet (StructFieldGet (Log) "d") #x #x.(Log.d');
-  #[global] Log_set_d (x : Log.t) y :: go.IsGoStepPureDet (StructFieldSet (Log) "d") (#x, #y) #(x <|Log.d' := y|>);
-  #[global] Log_get_l (x : Log.t) :: go.IsGoStepPureDet (StructFieldGet (Log) "l") #x #x.(Log.l');
-  #[global] Log_set_l (x : Log.t) y :: go.IsGoStepPureDet (StructFieldSet (Log) "l") (#x, #y) #(x <|Log.l' := y|>);
-  #[global] Log_get_cache (x : Log.t) :: go.IsGoStepPureDet (StructFieldGet (Log) "cache") #x #x.(Log.cache');
-  #[global] Log_set_cache (x : Log.t) y :: go.IsGoStepPureDet (StructFieldSet (Log) "cache") (#x, #y) #(x <|Log.cache' := y|>);
-  #[global] Log_get_length (x : Log.t) :: go.IsGoStepPureDet (StructFieldGet (Log) "length") #x #x.(Log.length');
-  #[global] Log_set_length (x : Log.t) y :: go.IsGoStepPureDet (StructFieldSet (Log) "length") (#x, #y) #(x <|Log.length' := y|>);
+  #[global] Log_get_d (x : Log.t) :: ⟦StructFieldGet (Logⁱᵐᵖˡ) "d", #x⟧ ⤳[under] #x.(Log.d');
+  #[global] Log_set_d (x : Log.t) y :: ⟦StructFieldSet (Logⁱᵐᵖˡ) "d", (#x, #y)⟧ ⤳[under] #(x <|Log.d' := y|>);
+  #[global] Log_get_l (x : Log.t) :: ⟦StructFieldGet (Logⁱᵐᵖˡ) "l", #x⟧ ⤳[under] #x.(Log.l');
+  #[global] Log_set_l (x : Log.t) y :: ⟦StructFieldSet (Logⁱᵐᵖˡ) "l", (#x, #y)⟧ ⤳[under] #(x <|Log.l' := y|>);
+  #[global] Log_get_cache (x : Log.t) :: ⟦StructFieldGet (Logⁱᵐᵖˡ) "cache", #x⟧ ⤳[under] #x.(Log.cache');
+  #[global] Log_set_cache (x : Log.t) y :: ⟦StructFieldSet (Logⁱᵐᵖˡ) "cache", (#x, #y)⟧ ⤳[under] #(x <|Log.cache' := y|>);
+  #[global] Log_get_length (x : Log.t) :: ⟦StructFieldGet (Logⁱᵐᵖˡ) "length", #x⟧ ⤳[under] #x.(Log.length');
+  #[global] Log_set_length (x : Log.t) y :: ⟦StructFieldSet (Logⁱᵐᵖˡ) "length", (#x, #y)⟧ ⤳[under] #(x <|Log.length' := y|>);
   #[global] Log_Apply_unfold :: MethodUnfold (Log) "Apply" (Log__Applyⁱᵐᵖˡ);
   #[global] Log_BeginTxn_unfold :: MethodUnfold (Log) "BeginTxn" (Log__BeginTxnⁱᵐᵖˡ);
   #[global] Log_Commit_unfold :: MethodUnfold (Log) "Commit" (Log__Commitⁱᵐᵖˡ);
