testdata/examples/go.mod
@@ -18,3 +18,5 @@ require (
 	golang.org/x/sys v0.29.0 // indirect
 	gopkg.in/yaml.v3 v3.0.1 // indirect
 )
+
+replace github.com/goose-lang/primitive => ./../../../primitive
